Deploying to gh-pages from @ xubaiw/reservoir-index@63a555515c23221b6c16dbc7987c8089f8bcad63 🚀

git/g4rgoil/tba-project/TBA/While/Solution.lean
@@ -1,8 +1,27 @@
 import TBA.While.Semantics
 
+import Aesop
+import TBA.Util.AesopExts
+
 namespace While
 
 namespace Optimisation
+
+
+
+
+-- Task 1: The semantic is deterministic.
+section task_1
+-- TODO
+theorem semDeterministic : ⟨c, σ⟩ ⇓ σ₁ : t₁ → ⟨c, σ⟩ ⇓ σ₂ : t₂ → ((∀ x, σ₁ x = σ₂ x) ∧  t₁ = t₂) := by
+  sorry
+end task_1
+
+
+
+
+-- Task 2: Formalisation of constant propagation and folding
+section task_2
 
 def foldExpr (σ : State) : Expr → Expr
   | .const v => Expr.const v
@@ -20,7 +39,7 @@ def foldExpr (σ : State) : Expr → Expr
 
 def foldCom (σ : State) : Com → (Com × State)
   | .skip => (Com.skip, σ)
-  | .ass x e => 
+  | .ass x e =>
       match foldExpr σ e with
       | .const v => (Com.ass x v, σ[x ↦ v])
       | e'       => (Com.ass x e', σ[x ↦ none])
@@ -28,7 +47,7 @@ def foldCom (σ : State) : Com → (Com × State)
     have (c₁', σ')  := foldCom σ c₁
     have (c₂', σ'') := foldCom σ' c₂
     (Com.seq c₁' c₂', σ'')
-  | .cond b cₜ cₑ => 
+  | .cond b cₜ cₑ =>
     match foldExpr σ b with
     | .const true  => foldCom σ cₜ
     | .const false => foldCom σ cₑ
@@ -42,6 +61,174 @@ def foldCom (σ : State) : Com → (Com × State)
 
 def optimise : Com → Com := λ c => (foldCom Map.empty c).1
 
+
+theorem Expr.custom_rec (p : Expr → Prop)
+    (htrue : p true) (hfalse : p  false) (hint : ∀ (x : Int), p x)
+    (hvar : ∀ (x : VName), p x) (hbinop : ∀ l op r, p (Expr.binop l op r))
+    : ∀ v, p v
+  | true | false | Val.int _ | .var _ | .binop .. => by simp_all
+
+end task_2
+
+
+
+
+-- Task 3: The optimisation preserves the semantics of a program.
+section task_3
+
+abbrev ConstMap (σ ρ : State) := ∀ x v, ρ x = some v → σ x = some v
+
+variable {c : Com} {e : Expr} {σ σ' ρ : State} {t : Nat}
+
+attribute [local simp] foldExpr
+
+theorem empty_ConstMap : ConstMap σ Map.empty := by
+  intro _ _ _; trivial
+
+theorem foldExprSound (h : ConstMap σ ρ) : Expr.eval σ e = Expr.eval σ (foldExpr ρ e) := by
+  induction e <;> aesop (add norm unfold Expr.eval)
+
+theorem foldCom_ConstMap (h : ConstMap σ ρ) (hc : ⟨c, σ⟩ ⇓ σ' : t)
+    : ConstMap σ' (foldCom ρ c).2 := by
+  induction hc generalizing ρ with
+    simp only [foldCom]
+  | skip => exact h
+  | ass => intro; aesop (add norm unfold Map.update, safe forward foldExprSound)
+  | seq _ _ ih₁ ih₂ => exact ih₂ (ih₁ h)
+  | ifTrue _ _ ih | ifFalse _ _ ih =>
+    cases hfold : foldExpr ρ ‹Expr› using Expr.custom_rec with
+    | htrue | hfalse =>
+      first | exact ih h | simp_all [foldExprSound h, Expr.eval]
+    | _ => intro _ _ _; rw [ih h]; aesop
+  | whileTrue =>
+    cases hfold : foldExpr ρ ‹Expr› using Expr.custom_rec with
+    | hfalse => simp_all [foldExprSound h, Expr.eval]
+    | _      => exact empty_ConstMap
+  | whileFalse => split <;> first | exact h | exact empty_ConstMap
+
+theorem foldExprEmpty (hfold : foldExpr Map.empty e = Expr.const v)
+    : foldExpr σ e = Expr.const v := by
+  induction e generalizing v with
+  | const => rw [←hfold]; rfl
+  | var x => simp_all [Map.empty]
+  | binop l op r ihl ihr =>
+    match hl : foldExpr Map.empty l, hr : foldExpr Map.empty r with
+    | .const _, .const _ => simp_all [ihl hl, ihr hr]
+    | .var _, _ | _, .var _ | .binop .., _ | _, .binop .. => simp_all
+
+theorem foldComSound (h : ConstMap σ ρ) (hc : ⟨c, σ⟩ ⇓ σ' : t)
+    : ∃ t', ⟨(foldCom ρ c).1, σ⟩ ⇓ σ' : t' := by
+  induction hc generalizing ρ with
+    simp only [foldCom]
+  | skip => exact ⟨1, Bigstep.skip⟩
+  | ass =>
+    rw [foldExprSound h]
+    cases foldExpr ρ ‹Expr› <;> exact ⟨_, Bigstep.ass⟩
+  | seq hc₁ _ ih₁ ih₂ =>
+    match ih₁ h, ih₂ (foldCom_ConstMap h hc₁) with
+    | ⟨_, h₁⟩, ⟨_, h₂⟩ => exact ⟨_, Bigstep.seq h₁ h₂⟩
+  | ifTrue hb _ ih | ifFalse hb _ ih =>
+    cases hfold : foldExpr ρ ‹Expr› using Expr.custom_rec with
+    | htrue | hfalse =>
+      first | exact ih h | simp_all [foldExprSound h, Expr.eval]
+    | _ =>
+      rw [foldExprSound h, hfold] at hb
+      have ⟨_, hc⟩ := ih h
+      first | exact ⟨_, Bigstep.ifTrue hb ‹_›⟩
+            | exact ⟨_, Bigstep.ifFalse hb ‹_›⟩
+  | whileTrue hb _ _ ihc ihind =>
+    rename Expr => b
+    cases hfold : foldExpr ρ b using Expr.custom_rec with
+    | hfalse => simp_all [foldExprSound h, Expr.eval]
+    | _ =>
+      cases hfold' : foldExpr Map.empty b using Expr.custom_rec with
+      | hfalse => simp_all [foldExprEmpty hfold']
+      | _ =>
+        have ⟨_, hc⟩ := ihc empty_ConstMap
+        have ⟨_, hind⟩ := ihind empty_ConstMap
+        rw [foldCom, hfold'] at hind
+        exact ⟨_, Bigstep.whileTrue hb hc hind⟩
+  | whileFalse hb =>
+    cases foldExpr ρ ‹Expr› using Expr.custom_rec with
+    | hfalse => exact ⟨_, Bigstep.skip⟩
+    | _      => exact ⟨_, Bigstep.whileFalse hb⟩
+
+-- Main prove that the constant propagation is sound (Task 3)
+theorem optimiseSound : ⟨c, σ⟩ ⇓ σ' : t → ∃ t', ⟨optimise c, σ⟩ ⇓ σ' : t' := 
+  foldComSound empty_ConstMap
+
+end task_3
+
+
+
+
+-- Task 4: The optimisation does not increase execution time.
+section task_4
+
+open Nat
+
+-- TODO: Make nicer
+theorem foldExprTime : (Expr.time (foldExpr σ e)) ≤ (Expr.time e) := by
+  induction e with simp only [foldExpr, Expr.time]
+  | var x => split <;> simp only [Expr.time]
+  | binop e₁ op e₂ h₁ h₂ =>
+    cases a : foldExpr σ e₁ with simp_all [Expr.time, add_le_add]
+    | const v₁ =>
+      cases b : foldExpr σ e₂ with simp_all [Expr.time, add_le_add]
+      | const v₂ =>
+        split
+        simp only [Expr.time, Nat.le_add_left 1 _]
+        simp only [Expr.time]
+        exact (Nat.add_le_add_right (Nat.add_le_add h₁ h₂) 1)
+
+
+variable {c : Com} {e : Expr} {σ σ' ρ : State} {t t₁ t₂ : Nat}
+
+attribute [local simp] foldExpr
+
+-- TODO: Formalize and prove
+theorem foldComTime : Prop := by
+  sorry
+
+end task_4
+
+
+
+
+-- Task 5: Constant propagation is idempotent.
+section task_5
+
+attribute [local simp] foldExpr
+attribute [local simp] foldCom
+
+theorem foldExprIdempotent : foldExpr σ (foldExpr σ e) = foldExpr σ e := by
+  induction e <;> aesop
+
+attribute [local simp] foldExprIdempotent
+
+
+-- TODO: Finalize proof
+theorem foldComIdempotent : foldCom σ ((foldCom σ c).1) = foldCom σ c := by
+  sorry
+
+
+theorem optimiseIdempotent : optimise (optimise c) = optimise c := by
+  simp_all [optimise]; aesop (add norm foldComIdempotent)
+
+end task_5
+
+
+
+
+-- Task 6: Formalize typing
+section task_6
+
+end task_6
+
+
+
+
 end Optimisation
+
 
 end While
