git/dupuisf/BibtexQuery/BibtexQuery/Entry.lean
@@ -1,0 +1,61 @@
+/-
+Copyright (c) 2022 Frédéric Dupuis. All rights reserved.
+Released under Apache 2.0 license as described in the file LICENSE.
+Author: Frédéric Dupuis
+-/
+
+import BibtexQuery.String
+
+/-!
+# Bibtex Entries and related functions
+
+This file defines inductive types for bibtex entries and tags, along with various related
+helper functions.
+-/
+
+namespace BibtexQuery
+
+/-- i.e. authors = "Binne, Chose and Truc, Machin" -/
+structure Tag where
+  Name : String
+  Content : String
+deriving Repr
+
+/-- A whole bibtex entry, i.e. a paper or a book. -/
+inductive Entry where
+  | NormalType (Class : String) (Name : String) (Tags : List Tag)
+  | StringType (Content : String)
+  | PreambleType (Content : String)
+  | CommentType
+deriving Repr
+
+namespace Entry
+
+/-- Returns the authors of a bibtex entry, or an empty string if it is not specified. -/
+def getAuthors : (e : Entry) → String
+| NormalType cl name tags =>
+  match tags.find? (fun t => t.Name = "author") with
+  | some t => t.Content
+  | none   => ""
+| _ => ""
+
+/-- Returns the title of a bibtex entry, or an empty string if it is not specified. -/
+def getTitle : (e : Entry) → String
+| NormalType cl name tags =>
+  match tags.find? (fun t => t.Name = "title") with
+  | some t => t.Content
+  | none   => ""
+| _ => ""
+
+/-- Returns the key of a bibtex entry. -/
+def getKey : Entry → String
+| NormalType cl name tags => name
+| _ => "No key"
+
+/-- Returns an abridged representation of a bibtex entry. -/
+def toAbridgedRepr (e : Entry) : String := 
+e.getKey.pad ' ' 25 ++ " | " ++ e.getAuthors.toLastNames.pad ' ' 50 ++ " | " ++ e.getTitle
+
+end Entry
+
+end BibtexQuery
