git/dupuisf/BibtexQuery/BibtexQuery/ParsecExtra.lean
@@ -1,0 +1,76 @@
+/-
+Copyright (c) 2022 Frédéric Dupuis. All rights reserved.
+Released under Apache 2.0 license as described in the file LICENSE.
+Author: Frédéric Dupuis
+-/
+
+import Lean.Data.Parsec
+
+/-!
+# Extra Parsec material
+
+This file contains additional material for the Parsec library, some of which is modelled after its Haskell
+counterpart.
+-/
+
+
+open Lean
+
+namespace Lean.Parsec
+
+def noneOf (bad : String) : Parsec Char := Parsec.satisfy (fun z => ¬bad.contains z)
+
+def noneOfStr (bad : String) : Parsec String := manyChars (noneOf bad)
+
+--def Lean.Parsec.line : Parsec String := Parsec.manyChars $ Parsec.noneOf '\n'
+
+def eol : Parsec String := 
+  Parsec.pstring "\n\r" <|> Parsec.pstring "\r\n" <|> Parsec.pstring "\n"
+
+partial def manyCore' (p : Parsec α) (acc : List α) : Parsec (List α) :=
+(do manyCore' p (acc ++ [←p])) <|> pure acc
+
+def many' (p : Parsec α) : Parsec (List α) := Parsec.manyCore' p []
+
+partial def manyStrCore (p : Parsec String) (acc : String) : Parsec String := 
+(do manyStrCore p (acc ++ (←p))) <|> pure acc
+
+def manyStr (p : Parsec String) : Parsec String := manyStrCore p ""
+
+partial def sepByCore (pcont : Parsec α) (psep : Parsec β) (acc : List α) : 
+  Parsec (List α) :=
+(do let _ ← psep; sepByCore pcont psep (acc ++ [←pcont])) <|> pure acc
+
+def sepBy (pcont : Parsec α) (psep : Parsec β) : Parsec (List α) :=
+do Parsec.sepByCore pcont psep [←pcont]
+
+partial def fuckme (p : Parsec α) : Parsec α := attempt p <|> fail "fukcme"
+
+partial def sepByCore' (pcont : Parsec α) (psep : Parsec β) (acc : List α) : 
+  Parsec (List α) := 
+attempt (do let _ ← psep; sepByCore' pcont psep (acc ++ [←pcont]))
+<|> (do  let _ ← attempt psep; return acc)
+<|> pure acc
+
+def sepBy' (pcont : Parsec α) (psep : Parsec β) : Parsec (List α) :=
+do Parsec.sepByCore' pcont psep [←pcont]
+
+partial def endByCore (pcont : Parsec α) (psep : Parsec β) (acc : List α) :
+  Parsec (List α) :=
+(do let x ← pcont; let _ ← psep; endByCore pcont psep (acc ++ [x])) <|> pure acc
+
+def endBy (pcont : Parsec α) (psep : Parsec β) : Parsec (List α) :=
+(do Parsec.endByCore pcont psep [])
+
+def asciiLetterToLower : Parsec Char := do return (←asciiLetter).toLower
+
+def asciiWordToLower : Parsec String := manyChars asciiLetterToLower
+
+def between (op : Parsec α) (cl : Parsec α) (mid : Parsec β) : Parsec β := do 
+  let _ ← op
+  let s ← mid
+  let _ ← cl
+  return s
+
+
+end Lean.Parsec
