git/dupuisf/BibtexQuery/BibtexQuery/Parser.lean
@@ -1,0 +1,114 @@
+/-
+Copyright (c) 2022 Frédéric Dupuis. All rights reserved.
+Released under Apache 2.0 license as described in the file LICENSE.
+Author: Frédéric Dupuis
+-/
+
+import BibtexQuery.ParsecExtra
+import BibtexQuery.Entry
+
+/-!
+# Bibtex Parser
+
+This file contains a parser for the Bibtex format. Note that currently, only a subset of the official
+Bibtex format is supported; features such as predefined strings and concatenation using `#` are not
+supported.
+-/
+
+open Lean Parsec
+
+namespace BibtexQuery.Parser
+
+/-- The name of the bibtex entry (i.e. what goes in the cite command). -/
+def name : Parsec String := do
+  let firstChar ← Parsec.asciiLetter
+  let reste ← manyChars $ (asciiLetter <|> digit <|> pchar ':' <|> pchar '-')
+  return firstChar.toString ++ reste
+
+/-- "article", "book", etc -/
+def classe : Parsec String := do skipChar '@'; asciiWordToLower
+
+partial def bracedContentAux (acc : String) : Parsec String :=
+(do let c ← anyChar
+    if c = '{' then
+      let s ← bracedContentAux ""
+      bracedContentAux (acc ++ s)
+    else
+      if c = '}' then return acc
+      else bracedContentAux (acc ++ c.toString))
+
+def bracedContent : Parsec String := do 
+  skipChar '{'
+  return ((←bracedContentAux "").replace "\n" "").replace "\r" ""
+
+def quotedContent : Parsec String := do 
+  skipChar '"'
+  let s ← manyChars $ noneOf "\""
+  skipChar '"'
+  return (s.replace "\n" "").replace "\r" ""
+
+def month : Parsec String := do 
+  let s ← asciiWordToLower
+  match s with
+  | "jan" => return s
+  | "feb" => return s
+  | "mar" => return s
+  | "apr" => return s
+  | "may" => return s
+  | "jun" => return s
+  | "jul" => return s
+  | "aug" => return s
+  | "sep" => return s
+  | "oct" => return s
+  | "nov" => return s
+  | "dec" => return s
+  | _     => fail "Not a valid month"
+
+/-- The content field of a tag. TODO: deal with months. -/
+def tagContent : Parsec String := do 
+  let c ← peek!
+  if c.isDigit then manyChars digit else
+    if c.isAlpha then month else
+      match c with
+      | '"' => quotedContent
+      | '{' => bracedContent
+      | _   => fail "Tag content expected"
+
+/-- i.e. journal = {Journal of Musical Deontology} -/
+def tag : Parsec Tag := do 
+  --let tagName ← asciiWordToLower
+  let tagName ← manyChars (asciiLetterToLower <|> pchar '_')
+  ws; skipChar '='; ws
+  let tagContent ← tagContent
+  return { Name := tagName, Content := tagContent }
+
+def outsideEntry : Parsec Unit := do let _ ← manyChars $ noneOf "@"
+
+/-- A Bibtex entry. TODO deal with "preamble" and all that crap. -/
+def entry : Parsec Entry := do 
+  outsideEntry
+  let typeOfEntry ← classe
+  ws; skipChar '{'; ws
+  let nom ← name
+  skipChar ','; ws
+  let t : List Tag ← sepBy' tag (do ws; skipChar ','; ws)
+  ws; skipChar '}'; ws
+  return Entry.NormalType typeOfEntry nom t
+
+def BibtexFile : Parsec (List Entry) := many' entry
+
+--#eval BibtexQuery.name "auTHOr23:z  ".mkIterator
+--#eval BibtexQuery.class "@ARTICLE ".mkIterator
+--#eval BibtexQuery.tag "auTHOr =   \n{Dès Noël où un zéphyr haï\n me vêt de glaçons würmiens, je dîne d'exquis rôtis de bœuf au kir à l'aÿ d'âge mûr}".mkIterator
+--#eval BibtexQuery.tag "auTHOr = \"Test\"".mkIterator
+--#eval BibtexQuery.tag "journal = {Journal of Musical\n Deontology}".mkIterator
+--#eval BibtexQuery.tag "year = 2022".mkIterator
+--#eval BibtexQuery.entry "  @article{bla23,\n year = 2022,\n author = {Frédéric Dupuis}\n}\n".mkIterator
+--#eval (Parsec.sepBy (manyChars $ Parsec.noneOf ",") (skipChar ',')) "bla, foo,".mkIterator
+
+--#eval (sepBy' asciiWordToLower (do ws; skipChar ','; ws)) "bla, foo, baz, ".mkIterator
+
+
+end BibtexQuery.Parser
+
+open Lean
