git/dupuisf/BibtexQuery/Main.lean
@@ -1,0 +1,92 @@
+/-
+Copyright (c) 2022 Frédéric Dupuis. All rights reserved.
+Released under Apache 2.0 license as described in the file LICENSE.
+Author: Frédéric Dupuis
+-/
+
+import Std.Data.HashMap
+import BibtexQuery.Parser
+import BibtexQuery.String
+import BibtexQuery.Query
+
+/-!
+# BibtexQuery: a simple command-line bibtex query utility
+
+BibtexQuery is a command-line utility that reads in a bibtex file and performs simple queries. A query is a string
+of the form "t.querystring", where `t` is either `a` for author, `t` for title or `k` for key, and `querystring`
+is a string (without spaces). BibtexQuery reads in a bibtex file, and returns the entries that match all the
+queries given a command-line parameters. Note that the entries are processed in such a way that strips diacritics,
+spaces and special characters before the queries are performed. In addition, the list of authors is normalized to
+firstnamelastname. Hence, for example, "Dupuis, Frédéric" will match the query `a.ericdup`.
+-/
+
+open Lean BibtexQuery
+
+def listDoublons (parseRes : List BibtexQuery.Entry) : List String :=
+  let keysOnly := parseRes.filterMap (fun entry => match entry with
+                                                   | BibtexQuery.Entry.NormalType _ name _ => some name
+                                                   | _ => none)
+  let ⟨hash, dupl⟩ : (Std.HashMap String Unit) × List String :=
+    keysOnly.foldl (init := ⟨Std.HashMap.empty, []⟩)
+      (fun ⟨hsh, lst⟩ key =>
+        match hsh.find? key with
+        | none => ⟨hsh.insert key (), lst⟩
+        | some _ => ⟨hsh, (key :: lst)⟩)
+  dupl
+
+def printHelp := IO.println 
+"
+bibtex-query - command-line bibtex file processor
+
+Usage: bibtex-query command filename [args]
+
+Commands:
+  h: print this help message
+  d: check for duplicate entries
+  l: list all entries in abridged form
+  q: print entries that match the given query
+
+Queries have the form «t.query» (without the quotes) with t being the type of query,
+and «query» being the content. The entries printed out are those that match all the queries.
+
+Types of queries:
+  k: key (ex: k.d14)
+  a: author (ex: a.dupuis)
+  t: title (ex: t.channelcapacity)
+"
+
+def printEntries (ents : List Entry) : IO Unit :=
+  for e in ents do
+    IO.println e.toAbridgedRepr
+
+def printMatchingEntries (ents : List Entry) (qs : List Query) : IO Unit := do
+  for e in ents do
+    if e.matchQueries qs then IO.println e.toAbridgedRepr 
+
+def main : List String → IO Unit
+| ["h"]           => printHelp
+| ["-h"]          => printHelp
+| ["--help"]      => printHelp
+| ["h", _]        => printHelp
+| ["-h", _]       => printHelp
+| ["--help", _]   => printHelp
+| ["d", fname]    => do
+  IO.println s!"Reading {fname} to find doubled keys"
+  let parsed := BibtexQuery.Parser.BibtexFile (←IO.FS.readFile fname).iter
+  match parsed with
+  | Parsec.ParseResult.success pos res => 
+    let lst := listDoublons res
+    IO.println lst
+  | Parsec.ParseResult.error pos err => IO.eprintln s!"Parse error at line {pos.lineNumber}: {err}"
+| ["l", fname]    => do
+  let parsed := BibtexQuery.Parser.BibtexFile (←IO.FS.readFile fname).iter
+  match parsed with
+  | Parsec.ParseResult.success pos res => printEntries res
+  | Parsec.ParseResult.error pos err => IO.eprint s!"Parse error at line {pos.lineNumber}: {err}"
+| "q" :: (fname :: queries) => do 
+  let parsed := BibtexQuery.Parser.BibtexFile (←IO.FS.readFile fname).iter
+  match parsed with
+  | Parsec.ParseResult.success pos res => printMatchingEntries res $ queries.filterMap Query.ofString
+  | Parsec.ParseResult.error pos err => IO.eprint s!"Parse error at line {pos.lineNumber}: {err}"
+| _            => do IO.eprintln "Invalid command-line arguments"; printHelp
+
